data/containers/rbtree/insert.lean
@@ -6,8 +6,10 @@ namespace rbtree
 open color
 
 /-- An insert_result is a generalization of the tree to allow
-temporaries tree-like structures that don't respect the red-black rules.
+a node with 2-keys and 3-children each of which should have the
+same height.
 
+This is used
 Specifically, it is either a tree that respects the red-black rules,
 or a the concatenation of three trees with the same height.
 -/
@@ -36,7 +38,6 @@ def as_tree : insert_result E → rbtree E
   | bin red ll lx lr := bin black (bin black ll lx lr) x (bin black c y r)
   | _ := bin black (bin red l x c) y r
   end
-
 
 def to_list : insert_result E → list E
 | (tree t) := t.to_list
@@ -76,10 +77,8 @@ def all_gt : insert_result E → E → Prop
 end
 end insert_result
 
-section
-parameters {E:Type _}
-
 section insert_def
+parameters {E:Type _}
 
 open insert_result
 
@@ -99,7 +98,7 @@ def balanceR : color → rbtree E → E → insert_result E → insert_result E
 -- black depth of the tree should not change.
 | co l x (triple rl rx rc ry rr) :=
   tree (bin red (bin black l x rl) rx (bin black rc ry rr))
-| co l x  (tree r) :=
+| co l x (tree r) :=
   match (co, r) with
   | (red, bin red rl rx rr) := triple l x rl rx rr
   | _ := tree (bin co l x r)
@@ -125,6 +124,7 @@ end insert_def
 -- to_list
 
 section to_list_theorems
+parameters {E:Type _}
 
 theorem to_list_balanceL (c : color) (l : insert_result E) (x : E) (r : rbtree E)
 : (balanceL c l x r).to_list  = l.to_list ++ [x] ++ r.to_list :=
@@ -144,6 +144,14 @@ begin
         cases c,
     };
   simp [*, balanceR, insert_result.to_list, to_list],
+end
+
+theorem to_list_as_tree (r : insert_result E)
+: r.as_tree.to_list = r.to_list :=
+begin
+  cases r with t tl tx tc ty tr;
+    try { cases tl with tlc tll tlx tlr;  try { cases tlc }, };
+    simp [insert_result.as_tree, rbtree.tree_color, insert_result.to_list, to_list],
 end
 
 parameters [has_preordering E]
@@ -184,21 +192,12 @@ begin
   },
 end
 
-theorem as_tree_to_list (r : insert_result E)
-: r.as_tree.to_list = r.to_list :=
-begin
-  cases r with t tl tx tc ty tr;
-    try { cases tl with tlc tll tlx tlr;  try { cases tlc },
-    };
-    simp [insert_result.as_tree, rbtree.tree_color, insert_result.to_list, to_list],
-end
-
 theorem to_list_insert (y : E) (t : rbtree E) : is_ordered t
  → to_list (insert y t)
     = t.to_list.filter (key_is_lt y) ++ y :: t.to_list.filter (key_is_gt y) :=
 begin
   intros,
-  simp [insert, as_tree_to_list, to_list_insert_core, *],
+  simp [insert, to_list_as_tree, to_list_insert_core, *],
 end
 
 theorem insert_eq (y : E)
@@ -218,6 +217,8 @@ end to_list_theorems
 -- is_ordered
 
 section is_ordered_theorems
+parameters {E:Type _}
+
 parameters [has_preordering E]
 local attribute [simp] balanceL balanceR insert_result.is_ordered is_ordered
   insert_result.all_lt all_lt insert_result.all_gt all_gt
@@ -226,7 +227,7 @@ local attribute [simp] balanceL balanceR insert_result.is_ordered is_ordered
 section balanceL
 parameters (c : color) (l : insert_result E) (y : E) (r : rbtree E)
 
-def all_lt_balanceL (a : E)
+theorem all_lt_balanceL (a : E)
   (all_lt_l : l.all_lt a)
   (y_lt_bnd : has_ordering.cmp y a = ordering.lt)
   (all_lt_r : all_lt r a)
@@ -237,7 +238,7 @@ begin
   try { simp at all_lt_l, simp [*], },
 end
 
-def all_gt_balanceL (a : E)
+theorem all_gt_balanceL (a : E)
   (iso : l.is_ordered)
   (a_lt_y : has_ordering.cmp a y = ordering.lt)
   (all_gt_l : l.all_gt a)
@@ -250,7 +251,7 @@ begin
   apply has_preordering.lt_of_lt_of_lt a tx ty; simp [*],
 end
 
-def is_ordered_balanceL
+theorem is_ordered_balanceL
   (l_iso : l.is_ordered)
   (all_lt_l_y : l.all_lt y)
   (all_gt_r_y : all_gt r y)
@@ -266,7 +267,7 @@ end balanceL
 section balanceR
 parameters (c : color) (l : rbtree E) (y : E) (r : insert_result E)
 
-def all_lt_balanceR (a : E)
+theorem all_lt_balanceR (a : E)
   (iso : r.is_ordered)
   (y_lt_a : has_ordering.cmp y a = ordering.lt)
   (all_lt_r_a : r.all_lt a)
@@ -279,8 +280,7 @@ begin
   apply has_preordering.lt_of_lt_of_lt tx ty a; simp [*],
 end
 
-
-def all_gt_balanceR (a : E)
+theorem all_gt_balanceR (a : E)
   (a_lt_y : has_ordering.cmp a y = ordering.lt)
   (all_gt_l : all_gt l a)
   (all_gt_r : r.all_gt a)
@@ -291,7 +291,7 @@ begin
   try { simp at all_gt_r, simp[*], },
 end
 
-def is_ordered_balanceR
+theorem is_ordered_balanceR
   (l_iso : is_ordered l)
   (all_lt_l_y : all_lt l y)
   (all_gt_r_y : r.all_gt y)
@@ -304,7 +304,16 @@ begin
 end
 end balanceR
 
-def insert_core_preserves (y : E) {t : rbtree E}
+theorem is_ordered_as_tree {r : insert_result E}
+  (iso : r.is_ordered)
+: r.as_tree.is_ordered :=
+begin
+  cases r with t tl tx tc ty tr;
+    try { cases tl with lc ll lx lr; try { cases lc}, };
+  simp at iso; simp [insert_result.as_tree, *],
+end
+
+theorem insert_core_preserves (y : E) {t : rbtree E}
   (iso : is_ordered t)
 : (insert_core y t).is_ordered
 ∧ (∀ (a : E), has_ordering.cmp y a = ordering.lt
@@ -366,20 +375,11 @@ begin
       { intros a a_lt_y pr,
         simp at pr,
         apply all_gt_balanceR; try { simp[*] },
-        apply r_all_gt; try {simp[*]},
-        apply all_gt_congr r a x; try {simp[*]},
+        apply r_all_gt; try { simp[*] },
+        apply all_gt_congr r a x; try { simp[*] },
       },
     },
   },
-end
-
-def as_tree_insert_result_ordered {r : insert_result E}
-  (iso : r.is_ordered)
-: r.as_tree.is_ordered :=
-begin
-  cases r with t tl tx tc ty tr;
-    try { cases tl with lc ll lx lr; try { cases lc}, };
-  simp at iso; simp [insert_result.as_tree, *],
 end
 
 theorem is_ordered_insert (y : E) (t : rbtree E)
@@ -387,12 +387,264 @@ theorem is_ordered_insert (y : E) (t : rbtree E)
 begin
   intro iso,
   simp [insert],
-  apply as_tree_insert_result_ordered,
+  apply is_ordered_as_tree,
   have h := insert_core_preserves y iso,
   simp[h],
 end
 end is_ordered_theorems
 
+-----------------------------------------------------------------------
+-- to_list
+
+
+namespace insert_result
+section
+parameters {E:Type _}
+
+def black_height : insert_result E → ℕ
+| (triple l _ _ _ _) := l.black_height
+| (tree t) := t.black_height
+
+def well_formed : insert_result E → Prop
+| (triple l x c y r) :=
+  l.well_formed
+  ∧ c.well_formed
+  ∧ r.well_formed
+  ∧ l.black_height = c.black_height
+  ∧ c.black_height = r.black_height
+  ∧ c.tree_color = black
+| (tree t) := t.well_formed
+
 end
+end insert_result
+
+section is_well_formed_theorems
+parameters {E:Type _}
+local attribute [simp] balanceL balanceR insert_result.well_formed well_formed
+  rbtree.tree_color insert_result.black_height black_height
+  insert_result.as_tree nat.add_succ
+  insert_core
+
+theorem succ_eq_succ (m n :ℕ) : (nat.succ m = nat.succ n) ↔ (m = n) :=
+  iff.intro nat.succ.inj (congr_arg nat.succ)
+
+local attribute [simp] succ_eq_succ
+
+theorem well_formed_balanceL_black (l : insert_result E) (x : E) (r : rbtree E)
+(l_wf : l.well_formed)
+(r_wf : r.well_formed)
+(l_ht_eq_r_ht : r.black_height = l.black_height)
+: (balanceL black l x r).well_formed  :=
+begin
+  cases l with t tl tx tc ty tr;
+    try { cases t with lc ll lx lr; try { cases lc } };
+    simp at l_wf l_ht_eq_r_ht;
+    simp [*],
+end
+
+theorem well_formed_balanceL_red (l : insert_result E) (x : E) (r : rbtree E)
+(l_wf : l.well_formed)
+(r_wf : r.well_formed)
+(l_ht_eq_r_ht : r.black_height = l.black_height)
+(r_black : r.tree_color = black)
+: (balanceL red l x r).well_formed  :=
+begin
+  cases l with t tl tx tc ty tr;
+    try { cases t with lc ll lx lr; try { cases lc } };
+    simp at l_wf;
+    simp [*],
+end
+
+theorem well_formed_balanceR_black (l : rbtree E) (x : E) (r : insert_result E)
+(l_wf : l.well_formed)
+(r_wf : r.well_formed)
+(l_ht_eq_r_ht : l.black_height = r.black_height)
+: (balanceR black l x r).well_formed  :=
+begin
+  cases r with t tl tx tc ty tr;
+    try { cases t with rc rl rx rr; try { cases rc } };
+    simp at r_wf;
+    simp [*],
+end
+
+theorem well_formed_balanceR_red (l : rbtree E) (x : E) (r : insert_result E)
+(l_wf : l.well_formed)
+(r_wf : r.well_formed)
+(l_ht_eq_r_ht : l.black_height = r.black_height)
+(l_black : l.tree_color = black)
+: (balanceR red l x r).well_formed  :=
+begin
+  cases r with t tl tx tc ty tr;
+    try { cases t with rc rl rx rr; try { cases rc } };
+    simp at r_wf;
+    try { simp [*], },
+end
+
+
+theorem black_height_balanceL_black (l : insert_result E) (x : E) (r : rbtree E)
+: (balanceL black l x r).black_height = l.black_height + 1 :=
+begin
+  cases l with t tl tx tc ty tr;
+    try { cases t with lc ll lx lr; try { cases lc } };
+    simp [*],
+end
+
+theorem black_height_balanceL_red (l : rbtree E) (x : E) (r : rbtree E)
+: (balanceL red (insert_result.tree l) x r).black_height = l.black_height :=
+begin
+  cases l with t tl tx tc ty tr;
+    try { cases t with lc ll lx lr; try { cases lc } };
+    simp [*],
+end
+
+theorem black_height_balanceR_black (l : rbtree E) (x : E) (r : insert_result E)
+: (balanceR black l x r).black_height = l.black_height + 1 :=
+begin
+  cases r with t tl tx tc ty tr;
+    try { cases t with rc rl rx rr; try { cases rc } };
+    simp [*],
+end
+
+theorem black_height_balanceR_red (l : rbtree E) (x : E) (r : rbtree E)
+: (balanceR red l x (insert_result.tree r)).black_height = l.black_height :=
+begin
+  cases r with t tl tx tc ty tr;
+    try { cases t with rc rl rx rr; try { cases rc } };
+    simp [*],
+end
+
+theorem well_formed_as_tree (r : insert_result E)
+: r.well_formed → r.as_tree.well_formed :=
+begin
+  intro r_wf,
+  cases r with t tl tx tc ty tr;
+    try { cases tl with tlc tll tlx tlr; try { cases tlc }, };
+    try { simp at r_wf, simp[r_wf], };
+    cc,
+end
+
+-- To simplify insert_core, we need a restricted definitions that work
+-- when the root node of the tree is colored black.  This allows us
+-- to make balanceL, balanceR, and insert_core return rbtrees rather
+-- that insert_result.
+section
+
+def balanceL_black : insert_result E → E → rbtree E → rbtree E
+| (insert_result.triple ll lx lc ly lr) x r :=
+  bin red (bin black ll lx lc) ly (bin black lr x r)
+| (insert_result.tree l) x r := bin black l x r
+
+def balanceR_black : rbtree E → E → insert_result E → rbtree E
+| l x (insert_result.triple rl rx rc ry rr) :=
+ bin red (bin black l x rl) rx (bin black rc ry rr)
+| l x (insert_result.tree r) := bin black l x r
+
+parameters [has_preordering E]
+
+def insert_core_black (y : E) : rbtree E → rbtree E
+| empty := bin red empty y empty
+| (bin c l x r) :=
+  match has_ordering.cmp y x with
+  | ordering.lt := balanceL_black (insert_core y l) x r
+  | ordering.eq := bin c l y r
+  | ordering.gt := balanceR_black l x (insert_core y r)
+  end
+
+theorem insert_core_black_eq (y : E) (t : rbtree E)
+: t.tree_color = black → insert_core y t = insert_result.tree (insert_core_black y t) :=
+begin
+  intro isb,
+  cases t with c l x r,
+  { simp [insert_core_black], },
+  { simp at isb,
+    destruct (has_ordering.cmp y x); intro cmp_y_x;
+      simp [*, insert_core_black],
+    { cases (insert_core y l); simp [balanceL_black], },
+    { cases (insert_core y r); simp [balanceR_black], },
+  },
+end
+end
+
+parameters [has_preordering E]
+
+local attribute [simp]
+  black_height_balanceL_black
+  black_height_balanceL_red
+  black_height_balanceR_black
+  black_height_balanceR_red
+
+theorem black_height_insert_core (y : E) (t : rbtree E)
+: t.well_formed → (insert_core y t).black_height = t.black_height :=
+begin
+  induction t,
+  case empty {
+    intros,
+    simp,
+  },
+  case bin c l x r l_ind r_ind {
+    cases c,
+    case red {
+      destruct (has_ordering.cmp y x); intro cmp_y_x; simp [cmp_y_x],
+      { intros l_wf r_wf l_isb r_isb l_ht_eq,
+        simp only [insert_core_black_eq y l l_isb, insert_result.black_height ] at l_ind,
+        simp only [*, insert_core_black_eq y l l_isb, black_height_balanceL_red],
+      },
+      { intros l_wf r_wf l_isb r_isb l_ht_eq,
+        simp only [*, insert_core_black_eq y r r_isb, black_height_balanceR_red],
+      },
+    },
+    case black {
+      destruct (has_ordering.cmp y x); intro cmp_y_x; simp [cmp_y_x],
+      { intros l_wf r_wf l_ht_eq,
+        simp only [*],
+      },
+    }
+  },
+end
+
+local attribute [simp] black_height_insert_core
+
+theorem well_formed_insert_core (y : E) (t : rbtree E)
+: t.well_formed → (insert_core y t).well_formed :=
+begin
+  induction t,
+  case empty {
+    intros,
+    simp,
+  },
+  case bin c l x r l_ind r_ind {
+    cases c,
+    case red {
+      destruct (has_ordering.cmp y x);
+        intro cmp_y_x;
+        simp [cmp_y_x];
+        intros,
+      { apply well_formed_balanceL_red; simp [*], },
+      { simp[*], },
+      { apply well_formed_balanceR_red; simp[*], },
+    },
+    case black {
+      destruct (has_ordering.cmp y x);
+        intro cmp_y_x;
+        simp [cmp_y_x];
+        intros,
+      { apply well_formed_balanceL_black; simp [*], },
+      { simp[*], },
+      { apply well_formed_balanceR_black; simp[*], },
+    }
+  },
+end
+
+theorem well_formed_insert (y : E) (t : rbtree E) : t.well_formed
+ → (insert y t).well_formed :=
+begin
+  intros,
+  apply well_formed_as_tree,
+  apply well_formed_insert_core,
+  assumption,
+end
+
+end is_well_formed_theorems
+
 end rbtree
 end data.containers
